src/cbor/CBOR.Spec.fst
@@ -1,0 +1,19 @@
+module CBOR.Spec
+open CBOR.Spec.Format
+module LPA = LowParse.SteelST.ArrayPtr.IntroElim
+module LPS = LowParse.SteelST.SeqMatch
+
+let serialize_cbor
+  c
+= LPS.serialize serialize_raw_data_item c
+
+let serialize_cbor_inj
+  c1 c2 s1 s2
+= LPS.parse_strong_prefix parse_raw_data_item (serialize_cbor c1) (serialize_cbor c1 `Seq.append` s1);
+  LPS.parse_strong_prefix parse_raw_data_item (serialize_cbor c2) (serialize_cbor c2 `Seq.append` s2);
+  LPS.serializer_injective _ serialize_raw_data_item c1 c2;
+  Seq.lemma_append_inj (serialize_cbor c1) s1 (serialize_cbor c2) s2
+
+let serialize_cbor_nonempty
+  c
+= ()
