src/cbor/CBOR.Spec.fsti
@@ -1,0 +1,22 @@
+module CBOR.Spec
+include CBOR.Spec.Type
+
+module U8 = FStar.UInt8
+
+(* Data format specification *)
+
+val serialize_cbor
+  (c: raw_data_item)
+: GTot (Seq.seq U8.t)
+
+val serialize_cbor_inj
+  (c1 c2: raw_data_item)
+  (s1 s2: Seq.seq U8.t)
+: Lemma
+  (requires (serialize_cbor c1 `Seq.append` s1 == serialize_cbor c2 `Seq.append` s2))
+  (ensures (c1 == c2 /\ s1 == s2))
+
+val serialize_cbor_nonempty
+  (c: raw_data_item)
+: Lemma
+  (Seq.length (serialize_cbor c) > 0)
